trunk/color/Util/Relation/GDomainBij.v
@@ -4,11 +4,9 @@ See the COPYRIGHTS and LICENSE files.
 
 - Leo Ducas, 2007-08-06
 
-GDomainBij
+Given a list Dom, we make a bijection between element of Dom and [[0,n-1]],
+and relation restricted to Dom with relation restricted to [[1,n]].
 *)
-
-(* given a list Dom, we make a bijection between element of Dom and [[0,n-1]],
-and relation restricted to Dom with relation restricted to [[1,n]] *)
 
 Set Implicit Arguments.
 
@@ -18,98 +16,65 @@ Require Export ListExtras.
 Require Export Path.
 Require Export Iter.
 Require Export AdjMat.
+
 Section Definitions.
+
 Variable A : Set.
-Variable A_eq_dec :forall (x:A) (y:A), {x=y} +{~x=y}.
+Variable eq_dec :forall x y : A, {x=y} + {~x=y}.
 Variable Dom : list A.
 Variable R : relation A.
-Variable R' :relation nat.
 
+(** Definition of the bijection of graphs *)
 
-(** Definition of the Bijection of graphs *)
-Definition domtonat x y:= 
- match Dom[x] with
- |None => False
- |Some a =>
-   match Dom[y] with
-   |None => False
-   |Some b => R a b
-   end
- end.
+Definition domtonat x y := 
+  match Dom[x] with
+    | None => False
+    | Some a =>
+      match Dom[y] with
+        | None => False
+        | Some b => R a b
+      end
+  end.
 
-Definition nattodom x y:=
-match list_find_first (eq x) (A_eq_dec x) Dom with
-  |None => False
-  |Some a =>
-  match list_find_first (eq y) (A_eq_dec y) Dom with
-   |None => False
-   |Some b => R' a b
-   end
- end.
+Variable R' : relation nat.
 
+Definition nattodom x y :=
+  match list_find_first (eq x) (eq_dec x) Dom with
+    | None => False
+    | Some a =>
+      match list_find_first (eq y) (eq_dec y) Dom with
+        | None => False
+        | Some b => R' a b
+      end
+  end.
 
 End Definitions.
 
 (** Some properties *)
+
 Section bijection.
 
-
-Lemma eq_In_find_first (A : Set) x l ( A_eq_dec :forall (x:A) (y:A), {x=y} +{~x=y}):
-In x l -> exists z, list_find_first (eq x) (A_eq_dec x) l = Some z /\ l[z]=Some x.
-intros; induction l.
-unfold In in H;tauto.
-simpl in H.
-destruct (A_eq_dec x a);subst.
-exists 0;split;simpl;auto with *.
-destruct (A_eq_dec a a); auto with *;tauto.
-destruct H;subst;try tauto.
-
-deduce (IHl H);destruct H0 as [z];destruct H0.
-exists (S z);split;simpl;auto with *.
-destruct (A_eq_dec x a);subst;try tauto.
-destruct (list_find_first (eq x) (A_eq_dec x) l);subst;try tauto;
-inversion H0;subst;auto.
-Qed.
-
-Lemma eq_list_find_first_exact (A : Set) l x z ( A_eq_dec :forall (x:A) (y:A), {x=y} +{~x=y}):
-list_find_first (eq x) (A_eq_dec x) l = Some z -> l[z]=Some x.
-Proof.
-intro;intro.
-induction l;intros;simpl in *. discriminate.
-destruct (A_eq_dec x a);subst.
-inversion H;subst;auto with *.
-
-assert (exists i,list_find_first (eq x) (A_eq_dec x) l=Some i).
-destruct (list_find_first (eq x) (A_eq_dec x) l);try discriminate.
-exists n0;auto with *.
-destruct H0.
-deduce(IHl _ _ _ H0).
-rewrite H0 in H.
-destruct z;inversion H;subst;assumption.
-Qed.
-
-
 Variable A : Set.
-Variable A_eq_dec :forall (x:A) (y:A), {x=y} +{~x=y}.
+Variable eq_dec :forall (x:A) (y:A), {x=y} +{~x=y}.
 Variable Dom : list A.
 Variable R : relation A.
 
-Lemma domtonat_elim  : forall a b, (domtonat Dom R) a b -> exists x,exists y,
-R x y /\ Dom [a] = Some x /\ Dom [b] = Some y.
-intros.
-unfold domtonat in H.
-destruct (Dom[a]);destruct (Dom[b]);try discriminate;try tauto.
-exists a0;exists a1;intuition; auto.
+Lemma domtonat_elim  : forall a b, domtonat Dom R a b ->
+  exists x, exists y, R x y /\ Dom [a] = Some x /\ Dom [b] = Some y.
+
+Proof.
+intros. unfold domtonat in H.
+destruct (Dom[a]); destruct (Dom[b]); try discriminate; try tauto.
+exists a0; exists a1; intuition; auto.
 Qed.
 
+Lemma domtonat_is_restricted :
+  is_restricted (domtonat Dom R) (nfirst_list (length Dom)).
 
-
-
-Lemma domtonat_is_restricted : is_restricted (domtonat Dom R) (nfirst_list (length Dom)).
 Proof.
-unfold is_restricted;intros.
-repeat rewrite nfirst_exact;deduce (domtonat_elim x y H).
-repeat destruct H0;destruct H1.
+unfold is_restricted; intros.
+repeat rewrite nfirst_exact; deduce (domtonat_elim x y H).
+repeat destruct H0; destruct H1.
 deduce(element_at_in2 _ _  H1).
 deduce(element_at_in2 _ _  H2).
 tauto.
@@ -117,87 +82,93 @@ Qed.
 
 Variable restriction : is_restricted R Dom.
 
-Lemma nattodom_elim :forall x y (R' : relation nat),
-nattodom A_eq_dec Dom (R') x y -> exists a, exists b,
-R' a b /\ Dom [a] = Some x /\ Dom [b] = Some y.
-intros;unfold nattodom in H.
-assert (exists a, list_find_first (eq x) (A_eq_dec x) Dom =Some a).
-destruct (list_find_first (eq x) (A_eq_dec x) Dom ); try tauto.
-exists n;auto. destruct H0; subst. rewrite H0 in H.
-assert (exists b,list_find_first (eq y) (A_eq_dec y) Dom =Some b).
-destruct (list_find_first (eq y) (A_eq_dec y) Dom ); try tauto.
-exists n;auto. destruct H1; subst;rewrite H1 in H.
+Lemma nattodom_elim : forall x y (R' : relation nat),
+  nattodom eq_dec Dom (R') x y ->
+  exists a, exists b, R' a b /\ Dom [a] = Some x /\ Dom [b] = Some y.
+
+Proof.
+intros; unfold nattodom in H.
+assert (exists a, list_find_first (eq x) (eq_dec x) Dom =Some a).
+destruct (list_find_first (eq x) (eq_dec x) Dom ); try tauto.
+exists n; auto. destruct H0; subst. rewrite H0 in H.
+assert (exists b,list_find_first (eq y) (eq_dec y) Dom =Some b).
+destruct (list_find_first (eq y) (eq_dec y) Dom ); try tauto.
+exists n; auto. destruct H1; subst; rewrite H1 in H.
 deduce(eq_list_find_first_exact _ _ _  H1).
 deduce(eq_list_find_first_exact _ _ _ H0).
-exists x0;exists x1;intuition;auto.
+exists x0; exists x1; intuition; auto.
 Qed.
-
 
 Lemma nattodom_elim2 :forall x y (R' : relation nat),
-nattodom A_eq_dec Dom (R') x y -> exists a, exists b,
-R' a b /\ list_find_first (eq x) (A_eq_dec x) Dom = Some a
-/\ list_find_first (eq y) (A_eq_dec y) Dom = Some b.
+  nattodom eq_dec Dom (R') x y ->
+  exists a, exists b, R' a b
+    /\ list_find_first (eq x) (eq_dec x) Dom = Some a
+    /\ list_find_first (eq y) (eq_dec y) Dom = Some b.
 
-intros;unfold nattodom in H.
-assert (exists a, list_find_first (eq x) (A_eq_dec x) Dom =Some a).
-destruct (list_find_first (eq x) (A_eq_dec x) Dom ); try tauto.
-exists n;auto. destruct H0; subst. rewrite H0 in H.
-assert (exists b,list_find_first (eq y) (A_eq_dec y) Dom =Some b).
-destruct (list_find_first (eq y) (A_eq_dec y) Dom ); try tauto.
-exists n;auto. destruct H1; subst;rewrite H1 in H.
+Proof.
+intros; unfold nattodom in H.
+assert (exists a, list_find_first (eq x) (eq_dec x) Dom =Some a).
+destruct (list_find_first (eq x) (eq_dec x) Dom ); try tauto.
+exists n; auto. destruct H0; subst. rewrite H0 in H.
+assert (exists b,list_find_first (eq y) (eq_dec y) Dom =Some b).
+destruct (list_find_first (eq y) (eq_dec y) Dom ); try tauto.
+exists n; auto. destruct H1; subst; rewrite H1 in H.
 deduce(eq_list_find_first_exact _ _ _ H1).
 deduce(eq_list_find_first_exact _ _ _ H0).
-exists x0;exists x1;intuition;auto.
+exists x0; exists x1; intuition; auto.
 Qed.
 
+Lemma dom_change: forall x y,
+  nattodom eq_dec Dom (domtonat Dom R) x y <-> R x y.
 
-Lemma dom_change:forall x y,
-nattodom A_eq_dec Dom (domtonat Dom R) x y <-> R x y.
-intros;split;intro.
+Proof.
+intros; split; intro.
 deduce (nattodom_elim _ _ _ H).
-repeat destruct H0;destruct H1.
+repeat destruct H0; destruct H1.
 unfold domtonat in H0.
-rewrite H1 in H0;rewrite H2 in H0;auto.
+rewrite H1 in H0; rewrite H2 in H0; auto.
 
 unfold is_restricted in restriction.
-deduce (restriction H);destruct H0.
-deduce (eq_In_find_first _ _  A_eq_dec H0);deduce (eq_In_find_first _ _ A_eq_dec H1).
-destruct H2;destruct H2;destruct H3;destruct H3.
+deduce (restriction H); destruct H0.
+deduce (eq_In_find_first eq_dec H0); deduce (eq_In_find_first eq_dec H1).
+destruct H2; destruct H2; destruct H3; destruct H3.
 unfold nattodom.
-rewrite H2;rewrite H3.
+rewrite H2; rewrite H3.
 unfold domtonat.
-rewrite H4;rewrite H5;auto.
+rewrite H4; rewrite H5; auto.
 Qed.
 
-Lemma domtonat_dec ( Rdec :forall x y, {R x y}+{~R x y}): forall x y,
-{domtonat Dom R x y}+{~(domtonat Dom R x y)}.
+Variable Rdec : forall x y, {R x y}+{~R x y}.
+
+Lemma domtonat_dec : forall x y, {domtonat Dom R x y}+{~domtonat Dom R x y}.
+
 Proof.
-intros.
-unfold domtonat.
-destruct (Dom[x]). destruct (Dom[y]). apply Rdec.
+intros. unfold domtonat. destruct (Dom[x]). destruct (Dom[y]). apply Rdec.
 tauto. tauto.
 Defined.
 
 End bijection.
 
-
-
 (** composition is mapped to composition *)
+
 Section compose.
+
 Variable A : Set.
-Variable A_eq_dec :forall (x:A) (y:A), {x=y} +{~x=y}.
+Variable eq_dec :forall (x:A) (y:A), {x=y} +{~x=y}.
 Variable Dom : list A.
 Variable R R': relation nat.
 Variable restriction : is_restricted R (nfirst_list (length Dom)).
 Variable restriction' : is_restricted R' (nfirst_list (length Dom)).
-Variable rp_free: repeat_free Dom.
+Variable rp_free : repeat_free Dom.
 
 Lemma dom_change_compose: forall x y,
-nattodom A_eq_dec Dom (R @ R') x y
-<-> ((nattodom A_eq_dec Dom R)@ nattodom A_eq_dec Dom R') x y.
-intros;split;intro.
-deduce (nattodom_elim A_eq_dec _ _ _ _ H).
-repeat destruct H0;destruct H1.
+  nattodom eq_dec Dom (R @ R') x y
+  <-> (nattodom eq_dec Dom R @ nattodom eq_dec Dom R') x y.
+
+Proof.
+intros; split; intro.
+deduce (nattodom_elim eq_dec _ _ _ _ H).
+repeat destruct H0; destruct H1.
 unfold compose; deduce (restriction H0); destruct H4.
 rewrite nfirst_exact in H5; rewrite element_at_exists in H5.
 destruct H5 as [z]; exists z.
@@ -208,159 +179,167 @@ unfold nattodom.
 destruct H6; clear H9.
 destruct H7; clear H9.
 destruct H8; clear H9.
-deduce (eq_In_find_first _ _ (A_eq_dec) H6);destruct H9;destruct H9.
-deduce (eq_In_find_first _ _ (A_eq_dec) H7); destruct H11; destruct H11.
-deduce (eq_In_find_first _ _ (A_eq_dec) H8);destruct H13;destruct H13.
+deduce (eq_In_find_first eq_dec H6); destruct H9; destruct H9.
+deduce (eq_In_find_first eq_dec H7); destruct H11; destruct H11.
+deduce (eq_In_find_first eq_dec H8); destruct H13; destruct H13.
 deduce (repeat_free_unique _ rp_free _ _ H1 H10).
 deduce (repeat_free_unique _ rp_free _ _ H3 H12).
 deduce (repeat_free_unique _ rp_free _ _ H5 H14).
-subst;rewrite H9;rewrite H11; rewrite H13;auto.
+subst; rewrite H9; rewrite H11; rewrite H13; auto.
 
-unfold compose in H; destruct H as [z];destruct H.
+unfold compose in H; destruct H as [z]; destruct H.
 unfold nattodom in *.
-destruct (list_find_first (eq x) (A_eq_dec x));auto with *.
-destruct (list_find_first (eq y) (A_eq_dec y));auto with *.
-destruct (list_find_first (eq z) (A_eq_dec z));auto with *.
-unfold compose;exists n1;auto with *.
+destruct (list_find_first (eq x) (eq_dec x)); auto with *.
+destruct (list_find_first (eq y) (eq_dec y)); auto with *.
+destruct (list_find_first (eq z) (eq_dec z)); auto with *.
+unfold compose; exists n1; auto with *.
 tauto.
-destruct (list_find_first (eq z) (A_eq_dec z));auto with *.
+destruct (list_find_first (eq z) (eq_dec z));auto with *.
 Qed.
 
 End compose.
 
-
 (** iteration mapped to iteration *)
+
 Section iter.
+
 Variable A : Set.
-Variable A_eq_dec :forall (x:A) (y:A), {x=y} +{~x=y}.
+Variable eq_dec :forall (x:A) (y:A), {x=y} +{~x=y}.
 Variable Dom : list A.
 Variable R : relation A.
 Variable restriction : is_restricted R Dom.
 Variable rp_free: repeat_free Dom.
 
 Lemma iter_preserv_restriction : forall n, is_restricted (iter R n) Dom.
-intro;induction n;try trivial.
-simpl;unfold is_restricted;unfold compose.
-intros;destruct H as [z];destruct H.
+
+Proof.
+intro; induction n; try trivial.
+simpl; unfold is_restricted; unfold compose.
+intros; destruct H as [z]; destruct H.
 intuition.
-deduce(restriction H);tauto.
-deduce(IHn _ _ H0);tauto.
+deduce(restriction H); tauto.
+deduce(IHn _ _ H0); tauto.
 Qed.
 
-
-
-
 Lemma dom_change_iter : forall n x y,
-nattodom A_eq_dec Dom (iter (domtonat Dom R) n) x y
-<-> (iter R n) x y.
-intro n; induction n;intros;simpl.
-apply dom_change;auto.
-split;intros.
+  nattodom eq_dec Dom (iter (domtonat Dom R) n) x y <-> iter R n x y.
+
+Proof.
+intro n; induction n; intros; simpl.
+apply dom_change; auto.
+split; intros.
 rewrite dom_change_compose in H.
 unfold compose in *.
-destruct H as [z];destruct H;exists z.
-rewrite dom_change in H;rewrite IHn in H0;auto with *.
+destruct H as [z]; destruct H; exists z.
+rewrite dom_change in H; rewrite IHn in H0; auto with *.
 apply domtonat_is_restricted.
 assumption.
 
-unfold compose in H;destruct H as [z];destruct H.
+unfold compose in H; destruct H as [z]; destruct H.
 rewrite dom_change_compose.
 apply domtonat_is_restricted.
-assumption. unfold compose;exists z;split.
-rewrite dom_change; assumption.
-rewrite IHn;assumption.
+assumption. unfold compose; exists z; split.
+rewrite dom_change;  assumption.
+rewrite IHn; assumption.
 Qed. 
 
-
-
-
 Lemma dom_change_tc: forall x y, 
-nattodom  A_eq_dec Dom ((domtonat Dom R)!) x y <-> R! x y.
+  nattodom eq_dec Dom (domtonat Dom R !) x y <-> R! x y.
 
-split;intros.
+Proof.
+split; intros.
 
-deduce(nattodom_elim2 A_eq_dec _ _ _ _ H);do 3 destruct H0.
-deduce (tc_iter H0);unfold Iter in *;unfold Iter_ge in *.
-destruct H2 as [n]. destruct H2;destruct H1.
-eapply (iter_tc R n);rewrite <- dom_change_iter.
-unfold nattodom;rewrite H1;rewrite H4;trivial.
+deduce(nattodom_elim2 eq_dec _ _ _ _ H); do 3 destruct H0.
+deduce (tc_iter H0); unfold Iter in *; unfold Iter_ge in *.
+destruct H2 as [n]. destruct H2; destruct H1.
+eapply (iter_tc R n); rewrite <- dom_change_iter.
+unfold nattodom; rewrite H1; rewrite H4; trivial.
 
-deduce (tc_iter H);unfold Iter in *;unfold Iter_ge in *.
-destruct H0 as [n];destruct H0.
+deduce (tc_iter H); unfold Iter in *; unfold Iter_ge in *.
+destruct H0 as [n]; destruct H0.
 rewrite <- dom_change_iter in H1.
 unfold nattodom in *.
-destruct (list_find_first (eq x) (A_eq_dec x) Dom);auto with *.
-destruct (list_find_first (eq y) (A_eq_dec y) Dom);auto with *.
-deduce (iter_tc (domtonat Dom R) n);auto.
+destruct (list_find_first (eq x) (eq_dec x) Dom); auto with *.
+destruct (list_find_first (eq y) (eq_dec y) Dom); auto with *.
+deduce (iter_tc (domtonat Dom R) n); auto.
 Qed.
 
 End iter.
 
 (** inteserction mapped to intersection *)
+
 Section intersection.
+
 Variable A : Set.
-Variable A_eq_dec :forall (x:A) (y:A), {x=y} +{~x=y}.
+Variable eq_dec :forall (x:A) (y:A), {x=y} +{~x=y}.
 Variable Dom : list A.
 Variable R R': relation nat.
 
-
 Lemma dom_change_inter : forall x y,
-nattodom A_eq_dec Dom (intersection R R') x y
-<-> (nattodom A_eq_dec Dom R) x y /\ (nattodom A_eq_dec Dom R') x y.
-split;intros;
+  nattodom eq_dec Dom (intersection R R') x y
+  <-> nattodom eq_dec Dom R x y /\ nattodom eq_dec Dom R' x y.
+
+Proof.
+split; intros;
 unfold nattodom in *;
-destruct (list_find_first (eq x) (A_eq_dec x) Dom);auto with *;
-destruct (list_find_first (eq y) (A_eq_dec y) Dom);auto with *.
+destruct (list_find_first (eq x) (eq_dec x) Dom);auto with *;
+destruct (list_find_first (eq y) (eq_dec y) Dom); auto with *.
 Qed.
 
 End intersection.
 
 (** transposition mapped to transposition *)
+
 Section transpose.
 Variable A : Set.
-Variable A_eq_dec :forall (x:A) (y:A), {x=y} +{~x=y}.
+
+Variable eq_dec :forall (x:A) (y:A), {x=y} +{~x=y}.
 Variable Dom : list A.
 Variable R : relation nat.
 
-
 Lemma dom_change_transp : forall x y,
-nattodom A_eq_dec Dom (transp R ) x y
-<-> transp (nattodom A_eq_dec Dom R) x y.
-split;intros;unfold transp in *;
+  nattodom eq_dec Dom (transp R) x y <-> transp (nattodom eq_dec Dom R) x y.
+
+Proof.
+split; intros; unfold transp in *;
 unfold nattodom in *;
-destruct (list_find_first (eq x) (A_eq_dec x) Dom);auto with *;
-destruct (list_find_first (eq y) (A_eq_dec y) Dom);auto with *.
+destruct (list_find_first (eq x) (eq_dec x) Dom); auto with *;
+destruct (list_find_first (eq y) (eq_dec y) Dom); auto with *.
 Qed.
 
 End transpose.
 
 (** SCC mapped to SCC *)
+
 Section domSCC.
+
 Variable A : Set.
-Variable A_eq_dec :forall (x:A) (y:A), {x=y} +{~x=y}.
+Variable eq_dec :forall (x:A) (y:A), {x=y} +{~x=y}.
 Variable Dom : list A.
 Variable R : relation A.
 Variable restriction : is_restricted R Dom.
 Variable rp_free: repeat_free Dom.
 
-
 Lemma dom_change_SCC : forall x y,
-nattodom  A_eq_dec Dom (SCC (domtonat  Dom R)) x y <-> SCC  R x y.
-split;intros;unfold SCC in *.
+  nattodom  eq_dec Dom (SCC (domtonat  Dom R)) x y <-> SCC  R x y.
+
+Proof.
+split; intros; unfold SCC in *.
 change ((R !) x y /\ transp (R !) x y).
-change (nattodom A_eq_dec Dom (intersection (domtonat Dom R !) 
+change (nattodom eq_dec Dom (intersection (domtonat Dom R !) 
 (transp (domtonat Dom R !))) x y) in H.
 rewrite dom_change_inter in H.
-destruct H;rewrite dom_change_transp in H0.
+destruct H; rewrite dom_change_transp in H0.
 unfold transp in *.
-rewrite dom_change_tc in *;auto with *.
+rewrite dom_change_tc in *; auto with *.
 
 change ((R !) x y /\ transp (R !) x y) in H.
-change (nattodom A_eq_dec Dom (intersection (domtonat Dom R !) 
+change (nattodom eq_dec Dom (intersection (domtonat Dom R !) 
 (transp (domtonat Dom R !))) x y).
 rewrite dom_change_inter.
-destruct H;rewrite dom_change_transp.
+destruct H; rewrite dom_change_transp.
 unfold transp in *.
-rewrite dom_change_tc;auto with *;rewrite dom_change_tc;auto with *.
+rewrite dom_change_tc; auto with *; rewrite dom_change_tc; auto with *.
 Qed.
+
 End domSCC.
